SystemF2r: start redoing kind environment

devel/Iron/Language/SystemF2r/Ki.v
@@ -4,13 +4,33 @@ Require Export Iron.Language.SystemF2r.Base.
 
 (* Kinds *)
 Inductive ki : Type :=
- | KStar   : ki
+ | KData   : ki
  | KFun    : ki -> ki -> ki.
 Hint Constructors ki.
 
 
 (* Kind Environments *)
 Definition kienv := list ki.
-Hint Unfold kienv.
+
+
+(* Kind env is the same as another, but with a new element. *)
+Definition keK      (k : ki)  (ke : kienv) (ke' : kienv) : Prop
+ := ke :> k  = ke'.
+
+
+(* Kind env is the same as another, but with a new element. *)
+Definition keKi     (i : nat) (k : ki)  (ke : kienv) (ke' : kienv) : Prop
+ := insert i k ke = ke'.
+
+
+(* Kind is the ith element of a kind environemnt. *)
+Definition keAtK    (i : nat) (ke : kienv) (k   : ki) : Prop
+ := get i ke = Some k.
+
+
+(* Get the size of a kind environment. *)
+Definition keSize (ke : kienv) : nat
+ := length ke.
+
 
 
