devel/Iron/Language/SystemF2r/SubstTypeType.v
@@ -7,51 +7,45 @@ Require Import Iron.Language.SystemF2r.KiJudge.
    otherwise indices that reference subst type are broken, and 
    the resulting type env would not be well formed *)
 Theorem subst_type_type_ix
- :  forall ix ke t1 k1 t2 k2
- ,  get ix ke = Some k2
- -> KIND ke t1 k1
- -> KIND (delete ix ke) t2 k2
- -> KIND (delete ix ke) (substTT ix t2 t1) k1.
+ :  forall ix ke ke' t1 k1 t2 k2
+ ,  keKi   ix k2 ke ke'
+ -> KIND ke' t1 k1
+ -> KIND ke  t2 k2
+ -> KIND ke  (substTT ix t2 t1) k1.
 Proof.
- intros. gen ix ke t2 k1 k2.
+ intros. gen ix ke ke' t2 k1 k2.
  induction t1; intros; simpl; inverts_kind; eauto.
 
  Case "TVar".
   fbreak_nat_compare.
   SCase "n = ix".
-   rewrite H in H4.
-   inverts H4. auto.
+   admit. (* ok, keKi keAtK lemma *)
 
   SCase "n < ix".
-   apply KIVar. rewrite <- H4.
-   apply get_delete_above; auto.
+   apply KIVar. 
+   admit. (* ok, need get_delete_above. *)
 
   SCase "n > ix".
-   apply KIVar. rewrite <- H4.
-   destruct n.
-    burn.
-    simpl. nnat. apply get_delete_below. omega.
+   apply KIVar.
+   admit. (* need get_delete_below. *)
 
  Case "TForall".
-  apply KIForall.
-  rewrite delete_rewind.
-  eapply IHt1; eauto.
-   apply kind_kienv_weaken; auto.
+  admit.
 Qed.
 
 
 Theorem subst_type_type_ix_forall2
- :  forall ix ke t2 k2 ts ks
- ,  get ix ke = Some k2
- -> Forall2 (KIND ke) ts ks
- ->          KIND (delete ix ke) t2 k2
- -> Forall2 (KIND (delete ix ke)) (map (substTT ix t2) ts) ks.
+ :  forall ix ke ke' t2 k2 ts ks
+ ,  keKi ix k2 ke ke'
+ -> Forall2 (KIND ke') ts ks
+ ->          KIND ke t2 k2
+ -> Forall2 (KIND ke) (map (substTT ix t2) ts) ks.
 Proof.
  intros.
  eapply Forall2_map_left.
  apply (Forall2_impl
-            (fun t k => KIND ke t k)
-            (fun t k => KIND (delete ix ke) (substTT ix t2 t) k)
+            (fun t k => KIND ke' t k)
+            (fun t k => KIND ke (substTT ix t2 t) k)
             ts ks).
   intros. eapply subst_type_type_ix; eauto.
   eauto.
@@ -59,14 +53,14 @@ Qed.
 
 
 Theorem subst_type_type
- :  forall ke t1 k1 t2 k2
- ,  KIND (ke :> k2) t1 k1
- -> KIND ke         t2 k2
+ :  forall ke ke' t1 k1 t2 k2
+ ,  keK k2 ke ke'
+ -> KIND ke' t1 k1
+ -> KIND ke  t2 k2
  -> KIND ke (substTT 0 t2 t1) k1.
 Proof.
  intros.
  unfold substTT.
- rrwrite (ke = delete 0 (ke :> k2)).
- eapply subst_type_type_ix; burn.
+ admit.
 Qed.
 
